Sodium/Crypto/Box.lean
@@ -1,12 +1,10 @@
-import Sodium.Theory.Basic
+import Sodium.Theory.Curve25519
 import Sodium.Data.Aead
-import Sodium.Data.Curve25519
-import Sodium.Data.Ristretto255
 import Sodium.Data.Core
 
 namespace Sodium.Crypto
 
-open Sodium.Theory
+open Theory
 
 def xsalsa20poly1305 : Aead where
   name := `xsalsa20poly1305
@@ -32,43 +30,8 @@ def aegis256 : Aead where
   encrypt := Aegis256.encrypt
   decrypt? := Aegis256.decrypt?
 
-def curve25519 : DhFunction where
-  name := `curve25519
-  scalarBytes := 32
-  pointBytes := 32
-  mulBase := Curve25519.mulBase
-  mul := Curve25519.mul
-
-def ristretto255Order : Nat := 2 ^ 252 + 27742317777372353535851937790883648493
-
-def ristretto255 : PrimeOrderGroup where
-  name := `ristretto255
-  scalarBytes := 32
-  pointBytes := 32
-  uniformBytes := 64
-  nonReducedBytes := 64
-  mulBase := Ristretto255.mulBase
-  mul := Ristretto255.mul
-  add := Ristretto255.add
-  sub := Ristretto255.sub
-  fromUniform := Ristretto255.fromHash
-  validPoint := Ristretto255.isValidPoint
-  scalarReduced s :=
-    decide (s.toByteArray.toList.foldr (fun b acc => b.toNat + 256 * acc) 0 < ristretto255Order)
-  scalarReduce := Ristretto255.scalarReduce
-  scalarAdd := Ristretto255.scalarAdd
-  scalarMul := Ristretto255.scalarMul
-  scalarNeg := Ristretto255.scalarNeg
-
-theorem curve25519_lawful : curve25519.Lawful := sorry
-theorem ristretto255_lawful : ristretto255.Lawful := sorry
-theorem xsalsa20poly1305_lawful : xsalsa20poly1305.Lawful := sorry
-
-def box : Box := dhBox curve25519 xsalsa20poly1305 hsalsa20
-def boxXchacha20poly1305 : Box := dhBox curve25519 xchacha20poly1305 hchacha20
-def boxRistretto255 : Box := dhBox ristretto255.toDhFunction xchacha20poly1305 blake2b32
-
-theorem box_lawful : box.Lawful :=
-  dhBox_lawful curve25519 xsalsa20poly1305 hsalsa20 curve25519_lawful xsalsa20poly1305_lawful
+def box : Box := dhBox Curve25519.spec xsalsa20poly1305 hsalsa20
+def boxXchacha20poly1305 : Box := dhBox Curve25519.spec xchacha20poly1305 hchacha20
+def boxRistretto255 : Box := dhBox Ristretto.spec.toDhFunction xchacha20poly1305 blake2b32
 
 end Sodium.Crypto
