Sodium/Crypto/Kdf.lean
@@ -1,0 +1,14 @@
+import Sodium.Theory.Basic
+import Sodium.Data.Kdf
+
+namespace Sodium.Crypto
+
+open Sodium.Theory
+
+def kdfBlake2b : Kdf where
+  name := `blake2b
+  keyBytes := 32
+  contextBytes := 8
+  derive := KdfBlake2b.derive
+
+end Sodium.Crypto
