Sodium/Crypto/Kx.lean
@@ -1,0 +1,14 @@
+import Sodium.Crypto.Box
+import Sodium.Data.GenericHash
+
+namespace Sodium.Crypto
+
+open Theory
+
+def kxKdf (q cpk spk : ByteVector 32) : ByteVector 32 × ByteVector 32 :=
+  let h := genericHash (q.toByteArray ++ cpk.toByteArray ++ spk.toByteArray)
+  (h.take 32 (by omega), (h.drop 32).cast (by omega))
+
+def kx : Kx := dhKx Curve25519.spec 32 kxKdf
+
+end Sodium.Crypto
