Sodium/Crypto/Sign.lean
@@ -1,0 +1,16 @@
+import Sodium.Crypto.Box
+import Sodium.Data.GenericHash
+
+namespace Sodium.Crypto
+
+open Theory
+
+def blake2b : Hash where
+  name := `blake2b
+  outBytes := 64
+  keyBytes := 32
+  hash := fun input key => genericHash input key
+
+def signRistretto255 : Sign := schnorr Ristretto.spec blake2b rfl
+
+end Sodium.Crypto
